use new wp fixedpoint

HeapLang/WeakestPrecondition.thy
@@ -4,16 +4,6 @@ begin
 
 subsection \<open>Weakest Preconditions\<close>
 
-function wp :: "stuckness \<Rightarrow> mask \<Rightarrow> expr \<Rightarrow> (val \<Rightarrow> iprop) \<Rightarrow> iprop" where
-  "wp s E e1 \<Phi> = (case HeapLang.to_val e1 of Some v \<Rightarrow> \<Turnstile>{E}=> (\<Phi> v)
-    | None \<Rightarrow> (\<forall>\<^sub>u \<sigma>1 \<kappa> \<kappa>s.
-      ((state_interp \<sigma>1 (\<kappa>@\<kappa>s)) ={E,Set.empty}=\<^emph>
-        ((\<upharpoonleft>(case s of NotStuck \<Rightarrow> reducible e1 \<sigma>1 | _ \<Rightarrow> True)) \<^emph>
-        (\<forall>\<^sub>u e2 \<sigma>2 efs. ((\<upharpoonleft>(prim_step e1 \<sigma>1 \<kappa> e2 \<sigma>2 efs))
-          ={Set.empty}\<triangleright>=\<^emph> (\<Turnstile>{Set.empty,E}=> ((state_interp \<sigma>2 \<kappa>s) \<^emph>
-            (wp s E e2 \<Phi>) \<^emph> ([\<^emph>\<^sub>l:] efs (\<lambda>ef. wp s UNIV ef (\<lambda>_. upred_emp)))))))))))"
-by auto
-
 lift_definition wp_pre :: "stuckness \<Rightarrow> ((mask \<Rightarrow> expr \<Rightarrow> (val \<Rightarrow> iprop) \<Rightarrow> iprop) -c>
   (mask \<Rightarrow> expr \<Rightarrow> (val \<Rightarrow> iprop) \<Rightarrow> iprop))" is
   "\<lambda>s wp_arg E e1 \<Phi>. (case HeapLang.to_val e1 of Some v \<Rightarrow> \<Turnstile>{E}=> (\<Phi> v)
@@ -27,11 +17,11 @@ apply (auto simp: contractive_alt_def contr_contr_alt n_equiv_fun_def split: opt
 apply (auto simp: ofe_refl less_Suc_eq_le ofe_mono intro!: upred_ne_rule contractiveE[OF upred_later_contr])
 by (simp add: n_equiv_fun_def ofe_mono)
 
-definition wp_def :: "stuckness \<Rightarrow> mask \<Rightarrow> expr \<Rightarrow> (val \<Rightarrow> iprop) \<Rightarrow> iprop" where
-  "wp_def s \<equiv> fixpoint (wp_pre s)"
+definition wp :: "stuckness \<Rightarrow> mask \<Rightarrow> expr \<Rightarrow> (val \<Rightarrow> iprop) \<Rightarrow> iprop" where
+  "wp s \<equiv> fixpoint (wp_pre s)"
 
-lemma wp_unfold: "wp_def s E e P \<stileturn>\<turnstile> Rep_contr (wp_pre s) (wp_def s) E e P"
-  unfolding wp_def_def using upred_eq_entails fixpoint_unfold[of "wp_pre s", unfolded ofe_eq_fun_def]
+lemma wp_unfold: "wp s E e P \<stileturn>\<turnstile> Rep_contr (wp_pre s) (wp s) E e P"
+  unfolding wp_def using upred_eq_entails fixpoint_unfold[of "wp_pre s", unfolded ofe_eq_fun_def]
   by blast
 
 abbreviation WP :: "expr \<Rightarrow> (val \<Rightarrow> iprop) \<Rightarrow> iprop" ("WP _ {{ _ }}") where
@@ -62,17 +52,14 @@ text \<open>
   First we show that some basic properties of wp hold for inputs in the domain, then we 
   always assume that all values lie in the domain.
 \<close>
-locale wp_rules =
-  assumes wp_dom_axiom: "wp_dom (s, E, e, P)"
-begin
-
-lemmas wp_simp = wp.psimps[OF wp_dom_axiom]
 
 lemma wp_value_fupd: "wp s E (of_val v) P \<stileturn>\<turnstile> \<Turnstile>{E}=> P v"
-  by (auto simp: wp_simp)
+  apply (rule upred_entail_eq_trans[OF wp_unfold])
+  by (simp add: wp_pre.rep_eq)
 
 lemma wp_value: "P v \<turnstile> wp s E (Val v) P"
-  by (auto simp: wp_simp fupd_intro upred_wand_holdsE)
+  apply (rule upred_entails_trans[OF _ upred_entail_eqR[OF wp_unfold]])
+  by (auto simp: wp_pre.rep_eq fupd_intro upred_wand_holdsE)
 
 lemma wp_fupd_helper: "\<forall>\<^sub>u v. (upred_emp ={E}=\<^emph> upred_emp)"
   apply (subst upred_holds_entails)
@@ -82,12 +69,14 @@ lemma wp_fupd_helper: "\<forall>\<^sub>u v. (upred_emp ={E}=\<^emph> upred_emp)"
 lemma wp_strong_mono: 
 assumes "s1 \<le> s2" 
 shows "\<forall>\<^sub>uE1 E2 e P Q. (\<upharpoonleft>(E1 \<subseteq> E2)) \<longrightarrow>\<^sub>u (wp s1 E1 e P -\<^emph> (\<forall>\<^sub>u v. (P v ={E2}=\<^emph> Q v)) -\<^emph> wp s2 E2 e Q)"
-  (is "upred_holds ?goal")  
+  (is "upred_holds ?goal")
   apply (rule loebI)
   apply (auto intro!: upred_forallI upred_implI_pure upred_wandI)
   subgoal for E1 E2 e P Q
-  apply (subst wp_simp[of _ E1])
-  apply (subst wp_simp[of _ E2])
+  apply (rule upred_entails_trans[OF _ upred_entail_eqR[OF wp_unfold]])
+  apply (move_sepL "wp s1 E1 e P")
+  apply (rule upred_entails_substE[OF upred_entail_eqL[OF wp_unfold]])
+  unfolding wp_pre.rep_eq
   apply (cases "HeapLang.to_val e")
   apply auto
   apply (auto intro!: upred_forallI upred_wandI)
@@ -95,14 +84,11 @@ shows "\<forall>\<^sub>uE1 E2 e P Q. (\<upharpoonleft>(E1 \<subseteq> E2)) \<lon
     apply (rule add_holds[OF fupd_mask_subseteq], assumption)
     apply (rule upred_entails_trans[OF _ fupd_mask_trans[of E2 E1]])
     apply (rule fupd_frame_mono)
-    apply (rule upred_entails_trans[OF upred_sep_comm2R])
-    apply (rule upred_entails_trans[OF upred_sep_comm4_2])
-    apply (rule upred_entails_trans[OF upred_sep_comm3M])
-    apply (rule upred_entails_trans[OF upred_sep_comm2R])
+    apply (move_sepL "\<forall>\<^sub>u (x::state). ?P x")
     apply (rule upred_entails_substE[OF upred_forall_inst[of _ \<sigma>1]])
     apply (rule upred_entails_substE[OF upred_forall_inst[of _ \<kappa>]])
     apply (rule upred_entails_substE[OF upred_forall_inst[of _ \<kappa>s]])
-    apply (rule upred_entails_substE[OF upred_wand_apply, unfolded upred_sep_assoc_eq])
+    apply iApply_wand
     apply (rule upred_entails_trans[OF _ fupd_mask_trans[of E1 "{}"]])
     apply (rule fupd_frame_mono)
     apply (simp add: upred_sep_assoc_eq)
@@ -187,7 +173,7 @@ shows "\<forall>\<^sub>uE1 E2 e P Q. (\<upharpoonleft>(E1 \<subseteq> E2)) \<lon
     apply (cases s1; cases s2)
     by auto
   subgoal for v
-    apply (rule upred_entails_substE[OF upred_forall_inst[of _ v]])
+    apply (iForallL v)
     apply (rule upred_wandE)
     apply (rule upred_entails_trans[OF _ fupd_ext])
   by (auto intro!: upred_entails_trans[OF upred_weakeningR] upred_wand_holdsE[OF fupd_mask_mono])
@@ -195,8 +181,9 @@ shows "\<forall>\<^sub>uE1 E2 e P Q. (\<upharpoonleft>(E1 \<subseteq> E2)) \<lon
 done
 
 lemma fupd_wp: "\<Turnstile>{E}=> (wp s E e P) \<turnstile> wp s E e P"
-  apply (subst wp_simp)
-  apply (subst wp_simp[of s E e P])
+  apply (rule upred_entails_trans[OF _ upred_entail_eqR[OF wp_unfold]])
+  apply(rule upred_entails_trans[OF fupd_mono[OF upred_entail_eqL[OF wp_unfold]]])
+  unfolding wp_pre.rep_eq
   apply (cases "HeapLang.to_val e")
   apply auto
   apply (auto intro!: upred_forallI)
@@ -241,7 +228,7 @@ shows "wp s E e P \<turnstile> wp s E e Q"
 lemma wp_mono':
 assumes "(\<And>v. P v \<turnstile> Q v)"
 shows "R \<^emph> wp s E e P \<turnstile> wp s E e Q"
-  using wp_mono[OF assms] assms upred_entails_trans upred_weakeningR wp_rules.wp_mono wp_rules_axioms 
+  using wp_mono[OF assms] assms upred_entails_trans upred_weakeningR wp_mono 
   by blast
 
 lemma wp_atomic: "atomic (stuckness_to_atomicity s) e \<Longrightarrow>
@@ -393,5 +380,4 @@ method iWP uses rule = iris_simp,
   ((entails_substR rule: fupd_intro | entails_substR rule: upred_laterI 
     | entails_substR rule: except_zeroI | entails_substR rule: updI)+)?,
   iApply rule: rule[simplified], iris_simp
-end  
-end   
+end
